\section{Pr\'{e}kopa--Leindler thoerem}

\begin{theorem}[Pr\'{e}kopa--Leindler]
    \label{thm:prekopa-leindler}
    \lean{PrekopaLeindler.prekopa_leindler}
    Let \(0<t<1\) be real and \(d\) be a nonnegative integer. Let \(f,g,h\colon \RR^d\to \RR\) be nonnegative integrable functions such that for all \(x,y\in \RR^d\),
    \begin{equation}\label{eq:prekopa-leindler_cond}
        f(x)^{1-t} g(y)^{t} \le h(x+y).
    \end{equation}
    Then
    \[
        \biggl( \int f(x) \diff x \biggr)^{\!1-t} \biggl( \int g(y) \diff y \biggr)^{\!t} \le (1-t)^{d(1-t)} t^{dt} \int h(x) \diff x.
    \]
\end{theorem}

\begin{lemma}
    \label{lem:prekopa-leindler-dimension-sum}
    If \Cref{thm:prekopa-leindler} holds for \(d=d_1\) and \(d_2\), then it also holds for \(d=d_1+d_2\).
\end{lemma}
\begin{proof}
    Let \(f,g,h\colon \RR^{d_1+d_2}\to \RR\) be nonnegative integrable functions which satisfy \eqref{eq:prekopa-leindler_cond}. We may regard them as the functions whose domains are \(\RR^{d_1}\times \RR^{d_2}\). Then for any \(x_1,y_1\in \RR^{d_1}\), the functions \(f(x_1,\cdot)\), \(g(y_1,\cdot)\), and \(h(x_1+y_1,\cdot)\) satisfy \eqref{eq:prekopa-leindler_cond} in dimension \(d_2\). Applying \Cref{thm:prekopa-leindler} for \(d=d_2\) yields that
    \begin{equation}\label{eq:FGH_cond}
        F(x_1)^{1-t} G(y_1)^{t}
        \le (1-t)^{d_2(1-t)} t^{d_2t} H(x_1+y_1),
    \end{equation}
    where
    \[
        F(x_1) \defeq \int f(x_1,\cdot) \diff x_2, \qquad
        G(y_1) \defeq \int g(y_1,\cdot) \diff y_2, \qquad
        H(z) \defeq \int h(z,\cdot) \diff z_2.
    \]
    Regarding \eqref{eq:FGH_cond} as the condition \eqref{eq:prekopa-leindler_cond} for \Cref{thm:prekopa-leindler}, we can apply the theorem for \(d=d_1\) using \(F\), \(G\), and \((1-t)^{d_2(1-t)} t^{d_2 t} H\). This gives
    \[
        \biggl( \int F(x) \diff x \biggr)^{\!1-t} \biggl( \int G(y) \diff y \biggr)^{\!t} 
        \le (1-t)^{d_1(1-t)} t^{dt} \int (1-t)^{d_2(1-t)} t^{d_2 t} H(x) \diff x.
    \]
    Unfolding the definitions of \(F\), \(G\), and \(H\), and applying the Fubini--Tonelli theorem complete the proof.
\end{proof}

\begin{corollary}
    If \Cref{thm:prekopa-leindler} holds for $d=1$, then it also holds for every $d\geq 1$.
\end{corollary}
\begin{proof}
    We prove by induction on $d$.
    The base case when $d=1$ is trivial, so suppose $d>1$.
    By induction, we know that \Cref{thm:prekopa-leindler} holds for dimension $d-1$ and $1$.
    Thus by \Cref{lem:prekopa-leindler-dimension-sum}, it becomes clear that \Cref{thm:prekopa-leindler} also holds for dimension $d$.
\end{proof}

\begin{lemma}[Pr\'ekopa--Leindler inequality in $\mathbb{R}$]
    \Cref{thm:prekopa-leindler} holds for $d=1$. In other words,
    if $f,g,h:\mathbb{R}\to\mathbb{R}$ are non-negative integrable functions which satisfy \Cref{eq:prekopa-leindler_cond},
    then
    \[\biggl( \int f(x) \diff x \biggr)^{\!1-t} \biggl( \int g(y) \diff y \biggr)^{\!t} \le (1-t)^{1-t} t^{t} \int h(x) \diff x\]
\end{lemma}
\begin{proof}
    Normalize $f$ and $g$ so that their sup norm becomes 1.
    Then the \href{https://en.wikipedia.org/wiki/Level_set}{super-level sets} satisfy
    \[\{\lambda<f\}+\{\lambda<g\}\subseteq\{\lambda<h\}\]
    as $\lambda=\lambda^{1-t}\lambda^{t}<f(x)^{1-t}g(y)^{t}\leq h(x+y)$ by \Cref{eq:prekopa-leindler_cond}.
    Also, \Cref{thm:one-dim} implies that $\mu(\{\lambda<f\})+\mu(\{\lambda<g\})\leq\mu(\{\lambda<h\})$ for every $\lambda\leq 1$.

    By the Fubini--Tonelli theorem,
    \[\int\phi(x)\diff x=\int_{0}^{\infty}\mu(\{\lambda<\phi\})\diff \lambda\]
    for $\phi\in\{f,g,h\}$.
    We thus obtain
    \begin{equation}
        \label{claim:int-ineq}
        \int f(x)\diff x+\int g(x)\diff x\leq \int h(x)\diff x
    \end{equation}

    Finally, the weighted AM-GM inequality implies that
    \begin{equation}
        \label{claim:am-gm-coro}
        \begin{split}
            a+b
            &=(1-t)\left(\frac{1}{1-t}a\right)+t\left(\frac{1}{t}b\right)\\
            &\leq\left(\frac{1}{1-t}a\right)^{1-t}\left(\frac{1}{t}b\right)^{t}\\
            &=\frac{1}{(1-t)^{1-t}t^{t}}a^{1-t}b^{t}
        \end{split}
    \end{equation}
    for any non-negative $a$ and $b$.
    Using \Cref{claim:int-ineq} and \Cref{claim:am-gm-coro} with $a=\int f(x)\diff x$ and $b=\int g(x)\diff x$, we get the desired inequality by transitivity of $\leq$.
\end{proof}
